theories/Crypt/Main.v
@@ -1,4 +1,5 @@
-From Crypt Require Import pkg_composition PRF ElGamal pkg_rhl UniformStateProb RulesStateProb.
+From Crypt Require Import pkg_composition PRF ElGamal pkg_rhl UniformStateProb
+  RulesStateProb.
 
 (* Notation to chain lets and end with 0 *)
 Notation "[ 'let' ]" :=
@@ -32,8 +33,8 @@ Definition results_from_the_paper := [let
   @Uniform_bij_rule ;
   @assert_rule ;
   @assert_rule_left ;
-  @bounded_do_while_rule;
-  @for_loop_rule;
+  @bounded_do_while_rule ;
+  @for_loop_rule ;
   Advantage_triangle ;
   Advantage_link ;
   @prove_relational ;
